add another mult algo and change the order of args

code/experimental/rsa/Addition.fst
@@ -9,8 +9,8 @@ module U32 = FStar.UInt32
 module U64 = FStar.UInt64
 
 val sub_loop:
-    aLen:bnlen -> bLen:bnlen ->
-    a:lbignum aLen -> b:lbignum bLen{disjoint a b} ->
+    aLen:bnlen -> a:lbignum aLen ->
+    bLen:bnlen -> b:lbignum bLen{disjoint a b} ->
     ind:U32.t{U32.v ind <= length a} -> carry:U64.t ->
     res:lbignum aLen{disjoint res a /\ disjoint res b} -> Stack unit
     (requires (fun h -> live h a /\ live h b /\ live h res))
@@ -19,7 +19,7 @@ val sub_loop:
 
 #set-options "--z3rlimit 150"
 
-let rec sub_loop aLen bLen a b ind carry res =
+let rec sub_loop aLen a bLen b ind carry res =
     if U32.(ind <^ aLen) then
         begin
         let t1 = a.(ind) in
@@ -31,19 +31,19 @@ let rec sub_loop aLen bLen a b ind carry res =
             else
                 (if U64.(t1 <^ t2) then 1uL else 0uL)) in
         let ind = U32.(ind +^ 1ul) in
-        sub_loop aLen bLen a b ind carry res
+        sub_loop aLen a bLen b ind carry res
         end
 
 (* a must be greater than b *)
 (* ADD: isMore aLen bLen a b *)
 (* res = a - b *)
 val sub:
-    aLen:bnlen -> bLen:bnlen ->
-    a:lbignum aLen -> b:lbignum bLen{disjoint a b} ->
+    aLen:bnlen -> a:lbignum aLen ->
+    bLen:bnlen -> b:lbignum bLen{disjoint a b} ->
     res:lbignum aLen{disjoint res a /\ disjoint res b} -> Stack unit
     (requires (fun h -> live h a /\ live h b /\ live h res))
 	(ensures (fun h0 _ h1 -> live h0 a /\ live h0 b /\  live h0 res /\
         live h1 a /\ live h1 b /\ live h1 res /\ modifies_1 res h0 h1))
 
-let sub aLen bLen a b res =
-    sub_loop aLen bLen a b 0ul 0uL res
+let sub aLen a bLen b res =
+    sub_loop aLen a bLen b 0ul 0uL res
