code/experimental/rsa/Shift.fst
@@ -7,66 +7,64 @@ open Lib
 
 module U32 = FStar.UInt32
 module U64 = FStar.UInt64
+open U32
 
 let bn_tbit = 0x8000000000000000uL
 
 val lshift_loop:
     aLen:bnlen ->
-    resLen:bnlen ->
     a:lbignum aLen ->
-    count:U32.t{U32.v count <= length a} ->
-    nw:U32.t -> lb:U32.t{0 < U32.v lb /\ U32.v lb < 64} ->
-    res:lbignum resLen{U32.v count + U32.v nw < length res /\ disjoint a res} -> 
-    Stack unit
+    count:U32.t ->
+    nw:U32.t ->
+    lb:U32.t{0 < v lb /\ v lb < 64} ->
+    res:lbignum aLen{v count + v nw < v aLen /\ disjoint a res} -> Stack unit
 	(requires (fun h -> live h a /\ live h res))
-	(ensures (fun h0 _ h1 -> live h0 a /\ live h0 res /\ 
+	(ensures (fun h0 _ h1 -> live h0 a /\ live h0 res /\
         live h1 a /\ live h1 res /\ modifies_1 res h0 h1))
 
-let rec lshift_loop aLen resLen a count nw lb res =
-    if U32.(count >^ 0ul) then begin
-        let ind = U32.(nw +^ count) in
+let rec lshift_loop aLen a count nw lb res =
+    if count >^ 0ul then begin
+        let ind = nw +^ count in
         let tmp = res.(ind) in
-        let count = U32.(count -^ 1ul) in
+        let count = count -^ 1ul in
         let t1 = a.(count) in
-        let rb = U32.(64ul -^ lb) in
-        assert(0 < U32.v rb /\ U32.v rb < 64);
+        let rb = 64ul -^ lb in
+        assert(0 < v rb /\ v rb < 64);
         res.(ind) <- U64.(tmp |^ U64.(t1 >>^ rb));
-        res.(U32.(ind -^ 1ul)) <- U64.(t1 <<^ lb);
-        lshift_loop aLen resLen a count nw lb res end
+        res.(ind -^ 1ul) <- U64.(t1 <<^ lb);
+        lshift_loop aLen a count nw lb res end
 
 (* res = a << n *)
 val lshift:
     aLen:bnlen ->
     a:lbignum aLen ->
-    nCount:U32.t{U32.v nCount > 0} ->
-    res:lbignum U32.(aLen +^ nCount /^ 64ul +^ 1ul){disjoint a res} ->
+    nCount:U32.t{v nCount > 0 /\ v aLen - (v nCount) / 64 - 1 > 0} ->
+    res:lbignum aLen{disjoint a res} ->
     Stack unit
 	(requires (fun h -> live h a /\ live h res))
 	(ensures (fun h0 _ h1 -> live h0 a /\ live h0 res /\
         live h1 a /\ live h1 res /\ modifies_1 res h0 h1))
 
 let lshift aLen a nCount res =
-    let nw = U32.(nCount/^ 64ul) in
-    let resLen = U32.(aLen +^ nw +^ 1ul) in
-    (**) assume(U32.v resLen > 0 /\ U32.v resLen <= 8192);
-    let lb = U32.(nCount %^ 64ul) in
-    (if U32.(lb =^ 0ul) then
-        blit a 0ul res nw aLen
-    else lshift_loop aLen resLen a aLen nw lb res)
+    let nw = nCount /^ 64ul in
+    let lb = nCount %^ 64ul in
+    (if lb =^ 0ul then
+        blit a 0ul res nw (aLen -^ nw)
+    else lshift_loop aLen a (aLen -^ nw -^ 1ul) nw lb res)
 
 val rshift1_loop:
     aLen:bnlen ->
     a:lbignum aLen ->
     carry:U64.t ->
-    ind:U32.t{U32.v ind < length a} ->
+    ind:U32.t{v ind < length a} ->
     res:lbignum aLen{disjoint a res} -> Stack unit
     (requires (fun h -> live h a /\ live h res))
 	(ensures (fun h0 _ h1 -> live h0 a /\ live h0 res /\ 
         live h1 a /\ live h1 res /\ modifies_1 res h0 h1))
 
 let rec rshift1_loop aLen a carry ind res =
-    if U32.(ind >^ 0ul) then begin
-        let ind = U32.(ind -^ 1ul) in
+    if ind >^ 0ul then begin
+        let ind = ind -^ 1ul in
         let tmp = a.(ind) in
         res.(ind) <- U64.((tmp >>^ 1ul) |^ carry);
         let carry = if U64.((tmp &^ 1uL) =^ 1uL) then bn_tbit else 0uL in
@@ -84,7 +82,7 @@ val rshift1:
 #set-options "--z3rlimit 50"
 
 let rshift1 aLen a res =
-    let i = U32.(aLen -^ 1ul) in
+    let i = aLen -^ 1ul in
     let tmp = a.(i) in
     let carry = if U64.((tmp &^ 1uL) =^ 1uL) then bn_tbit else 0uL in
     let tmp = U64.(tmp >>^ 1ul) in
