code/experimental/rsa/Comparison.fst
@@ -10,36 +10,32 @@ module U64 = FStar.UInt64
 module I32 = FStar.Int32
 
 val isMore_loop:
-    aLen:bnlen ->
-    bLen:bnlen{U32.v aLen = U32.v bLen} ->
-    a:lbignum aLen ->
-    b:lbignum bLen{disjoint a b} ->
+    aLen:bnlen -> a:lbignum aLen ->
+    bLen:bnlen{U32.v aLen = U32.v bLen} -> b:lbignum bLen{disjoint a b} ->
     count:U32.t{U32.v count <= length a} -> Stack bool
     (requires (fun h -> live h a /\ live h b))
 	(ensures (fun h0 _ h1 -> live h0 a /\ live h0 b
          /\ live h1 a /\ live h1 b /\ h0 == h1))
 
-let rec isMore_loop aLen bLen a b count =
+let rec isMore_loop aLen a bLen b count =
     if U32.(count >^ 0ul) then
         let count = U32.(count -^ 1ul) in
         let t1 = a.(count) in
         let t2 = b.(count) in
         (if not (U64.(t1 =^ t2)) then
             if U64.(t1 >^ t2) then true else false
-        else isMore_loop aLen bLen a b count)
+        else isMore_loop aLen a bLen b count)
     else false
 
 (* if a > b then true else false *)
 val isMore:
-    aLen:bnlen ->
-    bLen:bnlen ->
-    a:lbignum aLen ->
-    b:lbignum bLen{disjoint a b} -> Stack bool
+    aLen:bnlen -> a:lbignum aLen ->
+    bLen:bnlen -> b:lbignum bLen{disjoint a b} -> Stack bool
     (requires (fun h -> live h a /\ live h b))
     (ensures (fun h0 _ h1 -> live h0 a /\ live h0 b
         /\ live h1 a /\ live h1 b /\ h0 == h1))
 
-let isMore aLen bLen a b =
+let isMore aLen a bLen b =
     if U32.(aLen >^ bLen) then true
     else if U32.(aLen <^ bLen) then false
-         else isMore_loop aLen bLen a b aLen
+         else isMore_loop aLen a bLen b aLen
